rocq/theories/TypeSystem/TypeSafety.v
@@ -1256,55 +1256,9 @@ Lemma eval_direct_call_body_preserves_typing_prefix :
     store_ref_targets_preserved env
       (bind_params (fn_params fcall) vs s_args) s_body.
 Proof.
-  intros env Ω n Σ Σ_args fname args fdef fcall σ s s_args s_body
-    vs ret used' T_body Γ_out Hstore Hready_args Htyped_args Heval_args
-    Hlookup Henv_checked Henv_ready Hrename Htyped_body Hcompat_body
-    Heval_body.
-  destruct (proj1 (proj2 eval_preserves_typing_ready_mutual)
-              env s args s_args vs Heval_args Ω n Σ
-              (apply_lt_params σ (fn_params fdef)) Σ_args
-              Hready_args Hstore Htyped_args)
-    as [Hstore_args [Hargs_subst _]].
-  pose proof (alpha_rename_fn_def_shape (store_names s_args)
-                fdef fcall used' Hrename) as Hshape.
-  destruct Hshape as [_ [Hret Hparams_alpha]].
-  assert (Hargs_unsubst_fdef :
-    eval_args_values_have_types env Ω s_args vs (fn_params fdef)).
-  { eapply eval_args_values_have_types_apply_lt_params_inv.
-    exact Hargs_subst. }
-  assert (Hargs_fcall :
-    eval_args_values_have_types env Ω s_args vs (fn_params fcall)).
-  { eapply eval_args_values_have_types_params_alpha.
-    - exact Hparams_alpha.
-    - exact Hargs_unsubst_fdef. }
-  assert (Hnodup :
-    NoDup (ctx_names (params_ctx (fn_params fcall)))).
-  { eapply alpha_rename_fn_def_params_nodup_ctx_names. exact Hrename. }
-  assert (Hfresh : params_fresh_in_store (fn_params fcall) s_args).
-  { eapply alpha_rename_fn_def_params_fresh_in_store. exact Hrename. }
-  assert (Hstore_bind :
-    store_typed_prefix env (bind_params (fn_params fcall) vs s_args)
-      (sctx_of_ctx (params_ctx (fn_params fcall)))).
-  { eapply bind_params_store_typed_prefix; eassumption. }
-  assert (Hready_body : preservation_ready_expr (fn_body fcall)).
-  { eapply lookup_alpha_rename_fn_def_preservation_ready_body; eassumption. }
-  destruct (proj1 eval_preserves_typing_ready_prefix_mutual
-              env (bind_params (fn_params fcall) vs s_args)
-              (fn_body fcall) s_body ret Heval_body
-              (fn_outlives fcall) (fn_lifetimes fcall)
-              (sctx_of_ctx (params_ctx (fn_params fcall)))
-              T_body (sctx_of_ctx Γ_out)
-              Hready_body Hstore_bind Htyped_body)
-    as [Hstore_body [Hv_body Hpres_body]].
-  assert (Hv_ret_fcall : value_has_type env s_body ret (fn_ret fcall)).
-  { eapply value_has_type_compatible.
-    - exact Hv_body.
-    - apply ty_compatible_b_sound with (Ω := fn_outlives fcall).
-      exact Hcompat_body. }
-  assert (Hv_ret_fdef : value_has_type env s_body ret (fn_ret fdef)).
-  { rewrite Hret. exact Hv_ret_fcall. }
-  repeat split; try assumption.
-  eapply value_has_type_apply_lt_ty. exact Hv_ret_fdef.
+  eapply eval_direct_call_body_preserves_typing_prefix_with_preservation_core.
+  - exact eval_preserves_typing_ready_mutual.
+  - exact eval_preserves_typing_ready_prefix_mutual.
 Qed.
 
 Lemma eval_direct_call_body_preserves_typing_prefix_from_lookup :
@@ -1329,18 +1283,9 @@ Lemma eval_direct_call_body_preserves_typing_prefix_from_lookup :
       store_ref_targets_preserved env
         (bind_params (fn_params fcall) vs s_args) s_body.
 Proof.
-  intros env Ω n Σ Σ_args fname args fdef fcall σ s s_args s_body
-    vs ret used' Hstore Hready_args Htyped_args Heval_args Hlookup
-    Henv_checked Henv_ready Hrename Hcaps_call Heval_body.
-  pose proof (lookup_alpha_rename_fn_def_typed_structural
-                env fname fdef fcall (store_names s_args) used'
-                Hlookup Henv_checked Hrename) as Htyped_fn.
-  destruct (typed_fn_env_structural_body env fcall Htyped_fn)
-    as [T_body [Γ_out [Htyped_body [Hcompat_body _]]]].
-  rewrite (fn_body_ctx_eq_params_ctx_when_no_captures
-             fcall Hcaps_call) in Htyped_body.
-  exists Γ_out.
-  eapply eval_direct_call_body_preserves_typing_prefix; eassumption.
+  eapply eval_direct_call_body_preserves_typing_prefix_from_lookup_with_preservation_core.
+  - exact eval_preserves_typing_ready_mutual.
+  - exact eval_preserves_typing_ready_prefix_mutual.
 Qed.
 
 Theorem eval_preserves_typing_roots_ready_prefix_mutual :
